theories/CertiGC/model/heapgraph/remset/remset.v
@@ -2,10 +2,38 @@ From Coq Require Import Lists.List.
 From Coq Require Import micromega.Lia.
 From Coq Require Import ZArith.ZArith.
 
+From CertiGraph Require Import lib.List_ext.
+
 From CertiGC Require Import model.heapgraph.generation.generation.
 From CertiGC Require Import model.heapgraph.graph.
 
 Local Open Scope Z.
+
+Definition heapgraph_remember_upto (g : HeapGraph) (gen : nat): list Remember :=
+  fold_left
+    (fun rr g => rr ++ generation_remember g)
+    (firstn (S gen) (generations (heapgraph_generations g)))
+    nil.
+
+Lemma heapgraph_remember_upto__heapgraph_generations_append__old 
+  (g : HeapGraph) (gi : Generation) 
+  (gen : nat) (Hgen : heapgraph_has_gen g gen) :
+  heapgraph_remember_upto (heapgraph_generations_append g gi) gen = heapgraph_remember_upto g gen.
+Proof.
+  unfold heapgraph_remember_upto, heapgraph_generations_append, heapgraph_generation.
+  f_equal.
+  Opaque firstn.
+  simpl.
+  Transparent firstn.
+  rewrite firstn_app.
+  unfold heapgraph_has_gen in Hgen.
+  replace
+    (S gen - length (generations (heapgraph_generations g)))%nat
+    with O
+    by lia.
+  now rewrite app_nil_r.
+Qed.
+
 
 Definition heapgraph_remember_size
   (g : HeapGraph) (gen : nat) : Z :=
