theories/CertiGC/model/gc_correct.v
@@ -526,9 +526,10 @@ Proof.
       specialize (H3 _ Hto__from vidx (field_index e)).
       simpl in *.
       rewrite Ee in H3.
-      apply H3 ; try easy.
-      simpl.
-      congruence.
+      admit.
+      (* apply H3 ; try easy. *)
+      (* simpl. *)
+      (* congruence. *)
     - assert (~ InEither (dst g1 e) vpl). {
         intro. unfold InEither in H26. rewrite Heqp, in_app_iff in H26.
         destruct H26; auto. rewrite <- H8 in H26. destruct H26 as [_ ?].
@@ -540,7 +541,8 @@ Proof.
         simpl in H27.
         specialize (H2 _ H27 vidx eidx).
         simpl in H2.
-        now specialize (H2 H21).
+        admit.
+        (* now specialize (H2 H21). *)
       }
       rewrite !list_bi_map_not_In; auto.
       2: intro F; apply n; apply gepl_InEither in F; auto.
@@ -821,7 +823,7 @@ Proof.
       rewrite Heqp, in_app_iff. left; assumption.
   - simpl. destruct (elabel g1 e).
     destruct (elabel (remove_heapgraph_generation_ve g2 from) (emap e)). reflexivity.
-Qed.
+Admitted.
 
 (** Other graph relation is sound *)
 
@@ -2634,8 +2636,9 @@ Lemma no_edge2gen_bep: forall g roots from to,
 Proof.
   intros. red in H0 |-* . intros. destruct e as [[gen vidx] eidx]. simpl in *.
   subst gen. destruct H as [_ [? _]]. red in H. rewrite H in H1. apply H0 in H1.
-  now rewrite H3 in H1.
-Qed.
+  admit.
+  (* now rewrite H3 in H1. *)
+Admitted.
 
 Lemma fr_O_backward_edge_prop: forall from to p g1 g2 roots f_info,
     from <> to -> heapgraph_has_gen g1 to -> sound_gc_graph g1 -> no_dangling_dst g1 ->
@@ -3212,8 +3215,9 @@ Proof.
       destruct H4 as [_ [? _]]. rewrite valid_path_cons_iff in H4.
       destruct H4 as [? [[? _] _]]. destruct H as [? [? ?]]. red in H, H8, H9.
       rewrite H9 in *. destruct e as [[gen vidx] eidx]. simpl in *. subst r.
-      simpl in *. rewrite H8 in H7. apply H0; auto.
-Qed.
+      admit.
+      (* simpl in *. rewrite H8 in H7. apply H0; auto. *)
+Admitted.
 
 Lemma frr_sound: forall (g1 g2 : HeapGraph) from to f_info roots1 roots2,
     sound_gc_graph g1 -> heapgraph_has_gen g1 to ->
@@ -3357,10 +3361,11 @@ Proof.
   intros. red in H0. destruct (heapgraph_has_gen_dec g1 gen).
   - subst; auto.
   - destruct H0 as [gen_i [? ?]]. subst g2. unfold no_edge2gen, gen2gen_no_edge in *.
-    intros. simpl in *. destruct H2 as [H2 H3].
-    simpl in *. apply heapgraph_generations_append__heapgraph_has_block_inv in H2; auto.
-    rewrite <- ang_heapgraph_block_fields in H3. apply H; auto. split; auto.
-Qed.
+    admit.
+    (* intros. simpl in *. destruct H2 as [H2 H3]. *)
+    (* simpl in *. apply heapgraph_generations_append__heapgraph_has_block_inv in H2; auto. *)
+    (* rewrite <- ang_heapgraph_block_fields in H3. apply H; auto. split; auto. *)
+Admitted.
 
 Lemma ngr_iso: forall g1 g2 roots gen,
     new_gen_relation gen g1 g2 -> gc_graph_iso g1 roots g2 roots.
