theories/CertiGC/model/heapgraph/graph.v
@@ -11,7 +11,7 @@ From CertiGraph Require Import lib.List_ext.
 
 From CertiGC Require Import model.constants.
 From CertiGC Require Import model.util.
-From CertiGC Require Import vst.model.c_constants. (* uses WORD_SIZE *)
+From CertiGC Require Import vst.cmodel.constants. (* uses WORD_SIZE *)
 
 Import ListNotations.
 
