theories/CertiGC/vst/proof/verif_forward.v
@@ -9,8 +9,8 @@ From CertiGraph Require Import lib.List_ext.
 From CertiGC Require Import model.GCGraph.
 From CertiGC Require Import vst.ast.env_graph_gc.
 From CertiGC Require Import vst.clightgen.gc.
-From CertiGC Require Import vst.model.c_constants.
-From CertiGC Require Import vst.model.spatial_gcgraph.
+From CertiGC Require Import vst.cmodel.constants.
+From CertiGC Require Import vst.cmodel.spatial_gcgraph.
 From CertiGC Require Import vst.spec.gc_spec.
 
 Local Open Scope logic.
